filled hole in veric (no more yuck admits)
semax_func_cons_ext requires typechecking of the return value in terms
of C types (Clight.type), but the user is now provided with the fact
that the return value typechecks in terms of assembly types (AST.typ),
which in practice means no additional goal is generated.

sepcomp/step_lemmas.v
@@ -8,6 +8,13 @@ Require Import sepcomp.extspec.
 Require Import sepcomp.semantics.
 Require Import sepcomp.semantics_lemmas.
 
+Definition has_opttyp (v : option val) (t : option typ) :=
+  match v, t with
+    None, None => True
+  | Some v, Some t => Val.has_type v t
+  | _, _ => False
+  end.
+
 Section safety.
   Context {G C M Z:Type}.
   Context {genv_symb: G -> PTree.t block}.
@@ -28,7 +35,8 @@ Section safety.
       forall n z c m e args x,
       at_external Hcore c = Some (e,args) ->
       ext_spec_pre Hspec e x (genv_symb ge) (sig_args (ef_sig e)) args z m ->
-      (forall ret m' z' n',
+      (forall ret m' z' n'
+         (Hretty : has_opttyp ret (ef_sig e).(sig_res)),
          (n' <= n)%nat -> 
          Hrel n' m m' -> 
          ext_spec_post Hspec e x (genv_symb ge) (sig_res (ef_sig e)) ret z' m' ->
@@ -154,8 +162,8 @@ Section safety.
     + econstructor; eauto.
     + eapply safeN_external; eauto.
       rewrite <-H; auto.
-      intros ????? H8 H9.
-      specialize (H7 _ _ _ _ H3 H8 H9).
+      intros ???? Hretty ? H8 H9.
+      specialize (H7 _ _ _ _ Hretty H3 H8 H9).
       destruct H7 as [c' [? ?]].
       exists c'; split; auto.
     + eapply safeN_halted; eauto.
